# 3 Signals and Systems: Part II
This lecture introduces the unit step and unit impulse signals, then discusses system definitions and core properties. In addition, solutions to recommended and optional problems are included.

## Suggested Reading
- Section 2.4.1, The Discrete-Time Unit Step and Unit Impulse Sequences, pages 26-27
- Section 2.3.2, The Continuous-Time Unit Step and Unit Impulse Functions, pages 22-25
- Section 2.5, Systems, pages 35-39
- Section 2.6, Properties of Systems, pages 39-45

## I. Basic Signals: Unit Step and Unit Impulse
### 1. Discrete-Time Signals
#### Unit Step Sequence
$$u[n]= \begin{cases}1 & n \geq 0 \\ 0 & n<0\end{cases}$$
> TRANSPARENCY 3.1: Discrete-time unit step and unit impulse sequences

#### Unit Impulse Sequence (Unit Sample)
$$\delta[n]= \begin{cases}1 & n=0 \\ 0 & n \neq 0\end{cases}$$

#### Relationship Between Step and Impulse
- Impulse as the first backward difference of step
  $$\delta[n]=u[n]-u[n-1]$$
  > TRANSPARENCY 3.2: The unit impulse sequence as the first backward difference of the unit step sequence
- Step as the running sum of impulse
  $$u[n]=\sum_{m=-\infty}^{n} \delta[m]$$
  > TRANSPARENCY 3.3: The unit step sequence as the running sum of the unit impulse
- Step as superposition of delayed impulses
  $$u[n]=\sum_{k=0}^{\infty} \delta[n-k]$$
  > TRANSPARENCY 3.4: The unit step sequence expressed as a superposition of delayed unit impulses

### 2. Continuous-Time Signals
#### Unit Step Function
$$u(t)= \begin{cases}0 & t<0 \\ 1 & t>0\end{cases}$$
- Can be defined as the limit of a rectangular pulse \(u_\Delta(t)\) as \(\Delta \to 0\)
  $$u(t)=u_{\Delta}(t) \quad \text{as } \Delta \to 0$$
  > TRANSPARENCY 3.5: The continuous-time unit step function

#### Unit Impulse Function
- Defined as the derivative of the unit step
  $$\delta(t)=\frac{d u(t)}{d t}$$
- Derived from the limit of the pulse derivative \(\delta_\Delta(t)\) as \(\Delta \to 0\)
  $$\delta_{\Delta}(t)=\frac{du_{\Delta}(t)}{dt}, \quad \delta(t)=\delta_{\Delta}(t) \quad \text{as } \Delta \to 0$$
  > TRANSPARENCY 3.6: The definition of the unit impulse as the derivative of the unit step
  > TRANSPARENCY 3.7: Interpretation of the continuous-time unit impulse as the limiting form of a rectangular pulse which has unit area and for which the pulse width approaches zero

#### Key Properties of Continuous-Time Impulse
- Infinite height, zero width, unit area
- Step as the running integral of impulse
  $$u(t)=\int_{-\infty}^{t} \delta(\tau) d \tau$$
  > TRANSPARENCY 3.8: The unit step expressed as the running integral of the unit impulse

## II. System Definitions and Interconnections
### 1. System Definition
- **Continuous-time**: Maps input signal \(x(t)\) to output signal \(y(t)\)
- **Discrete-time**: Maps input sequence \(x[n]\) to output sequence \(y[n]\)
> TRANSPARENCY 3.9: Definition of a system

### 2. System Interconnections
#### Cascade Interconnection
- Output of the first system is the input of the second system
  $$x \to \text{System 1} \to x_2 \to \text{System 2} \to y$$
> TRANSPARENCY 3.10: Interconnection of two systems in cascade

#### Parallel Interconnection
- Same input is fed to two systems; outputs are summed
  $$x_1=x_2=x, \quad y=y_1+y_2$$
> TRANSPARENCY 3.11: Interconnection of two systems in parallel

#### Feedback Interconnection
- Output of the first system is fed back to the input of the second system; output of the second system is added to the original input
  $$x_1=x+y_2, \quad y=y_1, \quad x_2=y_1$$
> TRANSPARENCY 3.12: Feedback interconnection of two systems

## III. Core System Properties
### 1. Memoryless
- Output at any time depends only on the input at the same time
- **Example**: \(y(t)=(2+\sin t)x(t)\) is memoryless; \(y[n]=\sum_{k=-\infty}^n x[k]\) is not memoryless

### 2. Invertible
- A system has an inverse if distinct inputs produce distinct outputs
- **Example**: \(y(t)=x(2t)\) is invertible (\(x(t)=y(t/2)\)); \(y[n]=\sum_{k=-\infty}^\infty x[k]\) is not invertible

### 3. Causal
- Output at any time depends only on past and present inputs, not future inputs
- **Example**: \(y[n]=\sum_{k=-\infty}^n x[k]\) is causal; \(y(t)=x(2t)\) is not causal

### 4. Stable
- Bounded input produces bounded output
- **Example**: \(y(t)=(2+\sin t)x(t)\) is stable; \(y[n]=\sum_{k=-\infty}^n x[k]\) is not stable

### 5. Time-Invariant
- A time shift in the input leads to the same time shift in the output
- **Example**: \(y(t)=\frac{dx(t)}{dt}\) is time-invariant; \(y(t)=(2+\sin t)x(t)\) is not time-invariant

### 6. Linear
- Satisfies superposition principle: \(T[ax_1+bx_2]=aT[x_1]+bT[x_2]\)
- **Example**: \(y(t)=\frac{dx(t)}{dt}\) is linear; \(y[n]=\max\{x[n],x[n-1],...\}\) is not linear

## IV. Solutions to Recommended Problems
### S3.1
1.  \(x[n]= \delta[n] + \delta [n - 3]\)
    > Figure S3.1-1
2.  \(x[n] = u[n]-u[n- 5]\)
    > n: 0 1 2 3 4 5
    > Figure S3.1-2
3.  \(x [n]=\delta[n] + (-1) \delta[n -1]+(-1)^2\delta[n-2] +(-1)^3 \delta[n -3]\)
    > n: -5 0
    > Figure S3.1-3
4.  \(x(t)= u(t +3) - u(t - 3)\)
    > t: -3 0 3
    > Figure S3.1-4
5.  \(x(t) = \delta(t + 2)\)
    > Amplitude: 1; t: -2
    > Figure S3.1-5
6.  \(x(t)=e^{-t}u(t)\)
    > Amplitude: 1; t: 0
    > Figure S3.1-6

### S3.2
1.  h
2.  d
3.  b
4.  e
5.  a, f
6.  None

### S3.3
(a)
$$x[n]=\delta[n-1]-2 \delta[n-2]+3 \delta[n-3]-2 \delta[n-4]+\delta[n-5]$$

(b)
$$s[n]=-u[n+3]+4 u[n+1]-4 u[n-2]+u[n-4]$$

### S3.4
We are given Figure S3.4-1.
> \(x(t)\); Amplitude: 1; t: 1 2
> Figure S3.4-1

\(x(-t)\) and \(x(1-t)\) are as shown in Figures S3.4-2 and S3.4-3.
> \(x(-t)\); t: -1 -2 → Figure S3.4-2
> \(x(1-t)\); t: -1 1 → Figure S3.4-3

(a) \(u(t+1)-u(t-2)\) is as shown in Figure S3.4-4.
> t: 0 2 → Figure S3.4-4
> Hence, \(x(1-t)[u(t+1)-u(t-2)]\) → Figure S3.4-5

(b) \(-u(2-3 t)\) looks as in Figure S3.4-6.
> t: 2/3; Amplitude: -1 → Figure S3.4-6
> Hence, \(u(t+1)-u(2-3 t)\) → Figure S3.4-7
> So \(x(1-t)[u(t+1)-u(2-3 t)]\) → Figure S3.4-8

### S3.5
(a)
$$y[n]=x^{2}[n]+x[n]-x[n-1]$$

(b)
$$y[n]=x^{2}[n]+x[n]-x[n-1]$$

(c)
$$
\begin{aligned}
y[n] &= H[x[n]-x[n-1]] \\
&=x^{2}[n]+x^{2}[n-1]-2 x[n] x[n-1]
\end{aligned}
$$

(d)
$$
\begin{aligned}
y[n] &= G\left[x^{2}[n]\right] \\
&=x^{2}[n]-x^{2}[n-1]
\end{aligned}
$$

(e)
$$
\begin{aligned}
y[n] &= F[x[n]-x[n-1]] \\
&=2(x[n]-x[n-1])+(x[n-1]-x[n-2]) \\
&=2 x[n]-x[n-1]-x[n-2]
\end{aligned}
$$

(f)
$$
\begin{aligned}
y[n] &= G[2 x[n]+x[n-1]] \\
&=2 x[n]-x[n-1]-x[n-2]
\end{aligned}
$$

**Equivalence Conclusion**: (a) and (b) are equivalent; (e) and (f) are equivalent.

### S3.6
Refer to **Section III. Core System Properties** for detailed analysis of memoryless, linear, time-invariant, causal, invertible, and stable properties.

### S3.7
(a)
- \(H\) is an integrator, so \(H^{-1}\) is a differentiator:
  $$H^{-1}: y(t)=\frac{d x(t)}{d t}$$
- \(G: y(t)=x(2 t)\), so \(G^{-1}: y(t)=x(t / 2)\)

(b)
> \(z(t) \stackrel{F^{-1}}{\rightarrow} x(t)\); \(z(t) \stackrel{G^{-1} H^{-1}}{\rightarrow} x(t)\)
> Figure S3.7

## V. Solutions to Optional Problems
### S3.8
(a)
$$x_{2}(t)=x_{1}(t)-x_{1}(t-2)$$
> \(y_{2}(t) = y_{1}(t)-y_{1}(t - 2)\); t: 2 3 → Figure S3.8-1

(b)
$$x_{3}(t)=x_{1}(t)+x_{1}(t+1)$$
> \(y_{3}(t)=y_{1}(t)+y_{1}(t + 1)\); t: -1 0 1 2 → Figure S3.8-2

(c)
$$x(t)=u(t-1)-u(t-2)$$
> \(y(t)=e^{-(t-1)}u(t-1)+u(-t)+e^{-(t-2)} u(t-2) -u(1-t)\) → Figure S3.8-3

(d)
$$y[n]=3 y_{1}[n]-2 y_{2}[n]+2 y_{3}[n]$$
> n: 0 1 2 3; Amplitude: 3 3 4 → Figure S3.8-4

(e)
$$y_{2}[n]=y_{1}[n]+y_{1}[n-1]$$
> Figure S3.8-5
$$y_{3}[n]=y_{1}[n+1]$$
> Figure S3.8-6

(f)
$$y_{1}(t)=\pi+6 \cos (2 t)-47 \cos (5 t)+\sqrt{e} \cos (6 t)$$
$$x_{2}(t)=\frac{1+t^{10}}{1+t^{2}}=\sum_{n=0}^{4}\left(-t^{2}\right)^{n}$$
$$y_{2}(t)=1-\cos (2 t)+\cos (4 t)-\cos (6 t)+\cos (8 t)$$

### S3.9
(a)
(i) The system is linear (satisfies superposition principle).
(ii) The system is not time-invariant (verified by input shift example).

(b)
$$
\begin{aligned}
y(t) &=\sum_{n=-\infty}^{\infty} x(t) \delta(t-n T) \\
&=\sum_{n=-\infty}^{\infty} \cos (2 \pi t) \delta(t-n T)
\end{aligned}
$$
> Corresponding figures: S3.9-1 ~ S3.9-6

(c)
$$y(t)=\sum_{n=-\infty}^{\infty} e^{t} \cos (2 \pi t) \delta(t-n T)$$
> Corresponding figures: S3.9-7 ~ S3.9-12

### S3.10
(a) **True**: Cascade of linear time-invariant systems is linear time-invariant.
(b) **False**: Two nonlinear systems in cascade can be linear.
(c)
$$y[n]=x[n]+\frac{1}{4} x[n-1]$$
> Conclusion: Linear and time-invariant.
(d)
$$y[n]=a x[n+1]+b x[n]+c x[n-1]$$

### S3.11
(a) \(y[n]=x[n]+x[n-1]\) is linear and time-invariant.
(b) The modified system is linear but not time-invariant.

### S3.12
(a) Causality implies that equal inputs for \(t<t_0\) lead to equal outputs for \(t<t_0\).
(b) \(y(t)=x(t)x(t+1)\): nonlinear, noncausal system.
(c) \(y(t)=x(t)+1\): nonlinear, causal system.
(d) Proved equivalence between system invertibility and zero-input zero-output property.
(e) \(y[n]=x^2[n]\): nonlinear, non-invertible system.

---
MIT OpenCourseWare
[http://ocw.mit.edu](http://ocw.mit.edu)
Resource: Signals and Systems
Professor Alan V. Oppenheim

The following may not correspond to a particular course on MIT OpenCourseWare, but has been provided by the author as an individual learning resource.

For information about citing these materials or our Terms of Use, visit: [http://ocw.mit.edu/terms](http://ocw.mit.edu/terms)
