# 3 Signals and Systems: Part II
## Solutions to Recommended Problems
### S3.1
1.  \(x[n]= \delta[n] + \delta [n - 3]\)
    > Figure S3.1-1
2.  \(x[n] = u[n]-u[n- 5]\)
    > n: 0 1 2 3 4 5
    > Figure S3.1-2
3.  \(x [n]=\delta[n] + (-1) \delta[n -1]+(-1)^2\delta[n-2] +(-1)^3 \delta[n -3]\)
    > n: -5 0
    > Figure S3.1-3
4.  \(x(t)= u(t +3) - u(t - 3)\)
    > t: -3 0 3
    > Figure S3.1-4
5.  \(x(t) = \delta(t + 2)\)
    > Amplitude: 1
    > t: -2
    > Figure S3.1-5
6.  \(x(t)=e^{-t}u(t)\)
    > Amplitude: 1
    > t: 0
    > Figure S3.1-6

### S3.2
1.  h
2.  d
3.  b
4.  e
5.  a, f
6.  None

### S3.3
(a)
$$x[n]=\delta[n-1]-2 \delta[n-2]+3 \delta[n-3]-2 \delta[n-4]+\delta[n-5]$$

(b)
$$s[n]=-u[n+3]+4 u[n+1]-4 u[n-2]+u[n-4]$$

### S3.4
We are given Figure S3.4-1.
> \(x(t)\)
> Amplitude: 1
> t: 1 2
> Figure S3.4-1

\(x(-t)\) and \(x(1-t)\) are as shown in Figures S3.4-2 and S3.4-3.
> \(x(-t)\)
> t: -1 -2
> Figure S3.4-2
> \(x(1-t)\)
> t: -1 1
> Figure S3.4-3

(a) \(u(t+1)-u(t-2)\) is as shown in Figure S3.4-4.
> t: 0 2
> Figure S3.4-4

Hence, \(x(1-t)[u(t+1)-u(t-2)]\) looks as in Figure S3.4-5.
> Figure S3.4-5

(b) \(-u(2-3 t)\) looks as in Figure S3.4-6.
> t: 2/3
> Amplitude: -1
> Figure S3.4-6

Hence, \(u(t+1)-u(2-3 t)\) is given as in Figure S3.4-7.
> t: -1 2/3
> Amplitude: -1
> Figure S3.4-7

So \(x(1-t)[u(t+1)-u(2-3 t)]\) is given as in Figure S3.4-8.
> t: -1 1 2/3
> Amplitude: 1
> Figure S3.4-8

### S3.5
(a)
$$y[n]=x^{2}[n]+x[n]-x[n-1]$$

(b)
$$y[n]=x^{2}[n]+x[n]-x[n-1]$$

(c)
$$
\begin{aligned}
y[n] &= H[x[n]-x[n-1]] \\
&=x^{2}[n]+x^{2}[n-1]-2 x[n] x[n-1]
\end{aligned}
$$

(d)
$$
\begin{aligned}
y[n] &= G\left[x^{2}[n]\right] \\
&=x^{2}[n]-x^{2}[n-1]
\end{aligned}
$$

(e)
$$
\begin{aligned}
y[n] &= F[x[n]-x[n-1]] \\
&=2(x[n]-x[n-1])+(x[n-1]-x[n-2])
\end{aligned}
$$
$$y[n]=2 x[n]-x[n-1]-x[n-2]$$

(f)
$$
\begin{aligned}
y[n] &= G[2 x[n]+x[n-1]] \\
&=2 x[n]+x[n-1]-2 x[n-1]-x[n-2] \\
&=2 x[n]-x[n-1]-x[n-2]
\end{aligned}
$$

**Equivalence Conclusion**:
- (a) and (b) are equivalent
- (e) and (f) are equivalent

### S3.6
#### Memoryless
1.  \(y(t)=(2+\sin t) x(t)\) is memoryless. \(y(t)\) depends only on \(x(t)\) and not on prior values of \(x(t)\).
2.  \(y[n]=\sum_{k=-\infty}^{n} x[n]\) is not memoryless. \(y[n]\) depends on values of \(x[\cdot]\) before the time instant \(n\).
3.  \(y[n]=\max \{x[n], x[n-1], ..., x[-\infty]\}\) is clearly not memoryless.

#### Linear
1.  For \(y(t)=(2+\sin t) x(t)=T[x(t)]\)
    $$
    \begin{aligned}
    T\left[a x_{1}(t)+b x_{2}(t)\right] &=(2+\sin t)\left[a x_{1}(t)+b x_{2}(t)\right] \\
    &=a(2+\sin t) x_{1}(t)+b(2+\sin t) x_{2}(t) \\
    &=a T\left[x_{1}(t)\right]+b T\left[x_{2}(t)\right]
    \end{aligned}
    $$
    Conclusion: linear.
2.  For \(y(t)=x(2 t)=T[x(t)]\)
    $$
    \begin{aligned}
    T\left[a x_{1}(t)+b x_{2}(t)\right] &=a x_{1}(2 t)+b x_{2}(2 t) \\
    &=a T\left[x_{1}(t)\right]+b T\left[x_{2}(t)\right]
    \end{aligned}
    $$
    Conclusion: linear.
3.  For \(y[n]=\sum_{k=-\infty}^{\infty} x[k]=T[x[n]]\)
    $$
    \begin{aligned}
    T\left[a x_{1}[n]+b x_{2}[n]\right] &=a \sum_{k=-\infty}^{\infty} x_{1}[k]+b \sum_{k=-\infty}^{\infty} x_{2}[k] \\
    &=a T\left[x_{1}[n]\right]+b T\left[x_{2}[n]\right]
    \end{aligned}
    $$
    Conclusion: linear.
4.  \(y[n]=\sum_{k=-\infty}^{n} x[k]\) is linear (same reasoning as above).
5.  For \(y(t)=\frac{d x(t)}{d t}=T[x(t)]\)
    $$
    \begin{aligned}
    T\left[a x_{1}(t)+b x_{2}(t)\right] &=\frac{d}{d t}\left[a x_{1}(t)+b x_{2}(t)\right] \\
    &=a \frac{d x_{1}(t)}{d t}+b \frac{d x_{2}(t)}{d t}=a T\left[x_{1}(t)\right]+b T\left[x_{2}(t)\right]
    \end{aligned}
    $$
    Conclusion: linear.
6.  For \(y[n]=\max \{x[n], ..., x[-\infty]\}=T[x[n]]\)
    $$
    \begin{aligned}
    T\left[a x_{1}[n]+b x_{2}[n]\right] &=\max \left\{a x_{1}[n]+b x_{2}[n], ..., a x_{1}[-\infty]+b x_{2}[-\infty]\right\} \\
    &\neq a \max \left\{x_{1}[n], ..., x_{1}[-\infty]\right\}+b \max \left\{x_{2}[n], ..., x_{2}[-\infty]\right\}
    \end{aligned}
    $$
    Conclusion: not linear.

#### Time-invariant
1.  For \(y(t)=(2+\sin t) x(t)=T[x(t)]\)
    $$
    \begin{aligned}
    T\left[x\left(t-T_{0}\right)\right] &=(2+\sin t) x\left(t-T_{0}\right) \\
    &\neq y\left(t-T_{0}\right)=\left(2+\sin \left(t-T_{0}\right)\right) x\left(t-T_{0}\right)
    \end{aligned}
    $$
    Conclusion: not time-invariant.
2.  For \(y(t)=x(2 t)=T[x(t)]\)
    $$
    T\left[x\left(t-T_{0}\right)\right]=x\left(2 t-2 T_{0}\right) \neq x\left(2 t-T_{0}\right)=y\left(t-T_{0}\right)
    $$
    Conclusion: not time-invariant.
3.  For \(y[n]=\sum_{k=-\infty}^{\infty} x[k]=T[x[n]]\)
    $$
    T\left[x\left[n-N_{0}\right]\right]=\sum_{k=-\infty}^{\infty} x\left[k-N_{0}\right]=y\left[n-N_{0}\right]
    $$
    Conclusion: time-invariant.
4.  For \(y[n]=\sum_{k=-\infty}^{n} x[k]=T[x[n]]\)
    $$
    T\left[x\left[n-N_{0}\right]\right]=\sum_{k=-\infty}^{n} x\left[k-N_{0}\right]=\sum_{l=-\infty}^{n-N_{0}} x[l]=y\left[n-N_{0}\right]
    $$
    Conclusion: time-invariant.
5.  For \(y(t)=\frac{d x(t)}{d t}=T[x(t)]\)
    $$
    T\left[x\left(t-T_{0}\right)\right]=\frac{d}{d t} x\left(t-T_{0}\right)=y\left(t-T_{0}\right)
    $$
    Conclusion: time-invariant.

#### Causal
1.  For \(y(t)=x(2 t)\)
    \(y(1)=x(2)\). The value of \(y(\cdot)\) at time = 1 depends on \(x(\cdot)\) at a future time = 2.
    Conclusion: not causal.
2.  For \(y[n]=\sum_{k=-\infty}^{n} x[k]\)
    The value of \(y[\cdot]\) at any instant \(n\) depends only on the previous values of \(x[\cdot]\).
    Conclusion: causal.

#### Invertible
1.  \(y(t)=x(2 t)\) is invertible. The inverse is \(x(t)=y(t / 2)\).
2.  \(y[n]=\sum_{k=-\infty}^{\infty} x[k]\) is not invertible. Summation is not generally an invertible operation.
3.  \(y(t)=\frac{d x(t)}{d t}\) is invertible to within a constant.

#### Stable
1.  For \(y(t)=(2+\sin t) x(t)\): If \(|x(t)|<M\), \(|y(t)|<(2+\sin t) M\). Conclusion: stable.
2.  For \(y(t)=x(2 t)\): If \(|x(t)|<M\), \(|x(2 t)|<M\) and \(|y(t)|<M\). Conclusion: stable.
3.  For \(y[n]=\sum_{-\infty}^{n} x[k]\): If \(|x[k]| ≤M\), \(|y[n]| ≤M \cdot \sum_{-\infty}^{n} 1\) which is unbounded. Conclusion: not stable.

### S3.7
(a)
- Since \(H\) is an integrator, \(H^{-1}\) must be a differentiator.
  $$H^{-1}: y(t)=\frac{d x(t)}{d t}$$
- \(G: y(t)=x(2 t)\)
- \(G^{-1}: y(t)=x(t / 2)\)

(b)
> \(z(t) \stackrel{F^{-1}}{\rightarrow} x(t)\)
> \(z(t) \stackrel{G^{-1} H^{-1}}{\rightarrow} x(t)\)
> Figure S3.7

## Solutions to Optional Problems
### S3.8
(a)
$$x_{2}(t)=x_{1}(t)-x_{1}(t-2)$$
> \(y_{2}(t) = y_{1}(t)-y_{1}(t - 2)\)
> t: 2 3
> Figure S3.8-1

(b)
$$x_{3}(t)=x_{1}(t)+x_{1}(t+1)$$
> \(y_{3}(t)=y_{1}(t)+y_{1}(t + 1)\)
> t: -1 0 1 2
> Amplitude: 2
> Figure S3.8-2

(c)
$$x(t)=u(t-1)-u(t-2)$$
> \(y(t)=e^{-(t-1)}u(t-1)+u(-t)+e^{-(t-2)} u(t-2) -u(1-t)\)
> Amplitude: 1
> Figure S3.8-3

(d)
$$y[n]=3 y_{1}[n]-2 y_{2}[n]+2 y_{3}[n]$$
> n: 0 1 2 3
> Amplitude: 3 3 4
> Figure S3.8-4

(e)
$$y_{2}[n]=y_{1}[n]+y_{1}[n-1]$$
> \(y_{2}[n]\)
> n: 0 1 2 3 4 5
> Figure S3.8-5

$$y_{3}[n]=y_{1}[n+1]$$
> n: 0 1 2 3
> Figure S3.8-6

(f)
From linearity:
$$y_{1}(t)=\pi+6 \cos (2 t)-47 \cos (5 t)+\sqrt{e} \cos (6 t)$$
$$x_{2}(t)=\frac{1+t^{10}}{1+t^{2}}=\sum_{n=0}^{4}\left(-t^{2}\right)^{n}$$
$$y_{2}(t)=1-\cos (2 t)+\cos (4 t)-\cos (6 t)+\cos (8 t)$$

### S3.9
(a)
(i) The system is linear because
$$
\begin{aligned}
T\left[a x_{1}(t)+b x_{2}(t)\right] &=\sum_{n=-\infty}^{\infty}\left[a x_{1}(t)+b x_{2}(t)\right] \delta(t-n T) \\
&=a \sum_{n=-\infty}^{\infty} x_{1}(t) \delta(t-n T)+b \sum_{n=-\infty} x_{2}(t) \delta(t-n T) \\
&=a T\left[x_{1}(t)\right]+b T\left[x_{2}(t)\right]
\end{aligned}
$$

(ii) The system is not time-invariant. For example, let \(x_{1}(t)=\sin (2 \pi t / T)\). The corresponding output \(y_{1}(t)=0\). Now shift the input \(x_{1}(t)\) by \(\pi / 2\) to get
$$x_{2}(t)=\sin \left(\frac{2 \pi t}{T}+\frac{\pi}{2}\right)=\cos \left(\frac{2 \pi t}{T}\right)$$
The output is
$$y_{2}(t)=\sum_{n=-\infty}^{+\infty} \delta(t-n T) \neq y_{1}\left(t+\frac{\pi}{2}\right)=0$$

(b)
$$
\begin{aligned}
y(t) &=\sum_{n=-\infty}^{\infty} x(t) \delta(t-n T) \\
&=\sum_{n=-\infty}^{\infty} \cos (2 \pi t) \delta(t-n T)
\end{aligned}
$$
> \(\cos(2\pi t)\)
> t: 0
> Figure S3.9-1
> \(y(t)\), \(T = 1\)
> t: 0
> Figure S3.9-2
> \(y(t)\), \(T=1/2\)
> t: 0
> Figure S3.9-3
> \(y(t)\), \(T=1/4\)
> t: 0
> Amplitude: 1
> Figure S3.9-4
> \(y(t)\), \(T=1/8\)
> t: 0
> Amplitude: 1
> Figure S3.9-5
> \(y(t)\), \(T=1/16\)
> t: 0
> Figure S3.9-6

(c)
$$y(t)=\sum_{n=-\infty}^{\infty} e^{t} \cos (2 \pi t) \delta(t-n T)$$
> \(e^t\cos(2\pi t)\)
> t: 1/2
> Amplitude: 1
> Figure S3.9-7
> \(y(t)\), \(T = 1\)
> Amplitude: \(e^0=1\)
> Figure S3.9-8
> \(y(t)\), \(T=1/2\)
> Amplitude: \(e^0=1\), \(e^{1/2}\), \(e^{-1/2}\)
> Figure S3.9-9
> \(y(t)\), \(T=1/4\)
> Amplitude: \(e^0=1\), \(e^{1/4}\), \(e^{-1/4}\), \(e^{3/4}\), \(e^{-3/4}\)
> Figure S3.9-10
> \(y(t)\), \(T=1/8\)
> Figure S3.9-11
> \(y(t)\), \(T=1/16\)
> Amplitude: 2
> Figure S3.9-12

### S3.10
(a) **True**. To see that the system is linear, write
$$y_{2}(t)=T_{2}\left[T_{1}[x(t)]\right] \triangleq T[x(t)]$$
$$
\begin{aligned}
T_{1}\left[a x_{1}(t)+b x_{2}(t)\right] &=a T_{1}\left[x_{1}(t)\right]+b T_{1}\left[x_{2}(t)\right] \\
&\Rightarrow T_{2}\left[T_{1}\left[a x_{1}(t)+b x_{2}(t)\right]\right]=T_{2}\left[a T_{1}\left[x_{1}(t)\right]+b T_{1}\left[x_{2}(t)\right]\right] \\
&=a T_{2}\left[T_{1}\left[x_{1}(t)\right]\right]+b T_{2}\left[T_{1}\left[x_{2}(t)\right]\right] \\
&=a T\left[x_{1}(t)\right]+b T\left[x_{2}(t)\right]
\end{aligned}
$$
We see that the system is time-invariant from
$$
\begin{aligned}
T_{2}\left[T_{1}[x(t-T)]\right] &=T_{2}\left[y_{1}(t-T)\right] \\
&=y_{2}(t-T)
\end{aligned}
$$
$$T[x(t-T)]=y_{2}(t-T)$$

(b) **False**. Two nonlinear systems in cascade can be linear, as shown in Figure S3.10. The overall system is identity, which is a linear system.
> Reciprocal \(y(t)=x(t)\)
> \(x(t) \stackrel{\text{Reciprocal}}{\rightarrow} x(t)\)
> Figure S3.10

(c)
$$
\begin{aligned}
y[n] &=z[2 n]=w[2 n]+\frac{1}{2} w[2 n-1]+\frac{1}{4} w[2 n-2] \\
&=x[n]+\frac{1}{4} x[n-1]
\end{aligned}
$$
Conclusion: The system is linear and time-invariant.

(d)
$$
\begin{aligned}
y[n]=z[-n] &=a w[-n-1]+b w[-n]+c w[-n+1] \\
&=a x[n+1]+b x[n]+c x[n-1]
\end{aligned}
$$

### S3.11
(a) For \(y[n]=x[n]+x[n-1]=T[x[n]]\)
1.  The system is linear because
    $$
    \begin{aligned}
    T\left[a x_{1}[n]+b x_{2}[n]\right] &=a x_{1}[n]+a x_{1}[n-1]+b x_{2}[n]+b x_{2}[n-1] \\
    &=a T\left[x_{1}[n]\right]+b T\left[x_{2}[n-1]\right]
    \end{aligned}
    $$
2.  The system is time-invariant because
    $$
    \begin{aligned}
    T[x[n-N]] &=x[n-N]+x[n-1-N] \\
    &=y[n-N]
    \end{aligned}
    $$

(b) The system is linear (similar steps to part (a)). It is not time-invariant because
$$
\begin{aligned}
T[x[n-N]] &=x[n-N]+x[n-N-1]+x[0] \\
&\neq y[n-N]=x[n-N]+x[n-N-1]+x[-N]
\end{aligned}
$$

### S3.12
(a) To show that causality implies the statement, suppose \(x_{1}(t) \to y_{1}(t)\) and \(x_{2}(t) \to y_{2}(t)\), where \(y_{1}(t)\) and \(y_{2}(t)\) depend on \(x_{1}(t)\) and \(x_{2}(t)\) for \(t<t_{0}\). By linearity:
$$x_{1}(t)-x_{2}(t) \to y_{1}(t)-y_{2}(t)$$
If \(x_{1}(t)=x_{2}(t)\) for \(t<t_{0}\), then \(y_{1}(t)=y_{2}(t)\) for \(t<t_{0}\). Hence, if \(x(t)=0\) for \(t<t_{0}\), \(y(t)=0\) for \(t<t_{0}\).

(b) \(y(t)=x(t) x(t+1)\)
- If \(x(t)=0\) for \(t<t_{0}\), then \(y(t)=0\) for \(t<t_{0}\).
- Conclusion: nonlinear, noncausal system.

(c) \(y(t)=x(t)+1\) is a nonlinear, causal system.

(d) We want to show the equivalence of the following two statements:
- **Statement 1 (S1)**: The system is invertible.
- **Statement 2 (S2)**: The only input that produces the output \(y[n]=0\) for all \(n\) is \(x[n]=0\) for all \(n\).

To show the equivalence, we will show that \(S2 \text{ false} \Rightarrow S1 \text{ false}\) and \(S1 \text{ false} \Rightarrow S2 \text{ false}\):
1. \(S2 \text{ false} \Rightarrow S1 \text{ false}\): Let \(x[n] \neq0\) produce \(y[n]=0\). Then \(c x[n] \Rightarrow y[n]=0\).
2. \(S1 \text{ false} \Rightarrow S2 \text{ false}\): Let \(x_{1} \Rightarrow y_{1}\) and \(x_{2} \to y_{2}\). If \(x_{1} \neq x_{2}\) but \(y_{1}=y_{2}\), then \(x_{1}-x_{2} \neq0\) but \(y_{1}-y_{1}=0\).

(e) \(y[n]=x^{2}[n]\) is nonlinear and not invertible.

---
MIT OpenCourseWare
[http://ocw.mit.edu](http://ocw.mit.edu)
Resource: Signals and Systems
Professor Alan V. Oppenheim

The following may not correspond to a particular course on MIT OpenCourseWare, but has been provided by the author as an individual learning resource.

For information about citing these materials or our Terms of Use, visit: [http://ocw.mit.edu/terms](http://ocw.mit.edu/terms)