# Introduction Solutions to Recommended Problems
## S1.1
1.  Using Euler's formula,
    $$e^{j \pi / 4}=\cos \frac{\pi}{4}+j \sin \frac{\pi}{4}=\frac{\sqrt{2}}{2}+j \frac{\sqrt{2}}{2}$$
    Since \(z=\frac{1}{2} e^{j \pi / 4}\)
    $$\operatorname{Re}\{z\}=\frac{1}{2} \operatorname{Re}\left\{\frac{\sqrt{2}}{2}+j \frac{\sqrt{2}}{2}\right\}=\frac{\sqrt{2}}{4}$$
2.  Similarly,
    $$\operatorname{Im}\{z\}=\frac{1}{2} \operatorname{Im}\left\{\frac{\sqrt{2}}{2}+j \frac{\sqrt{2}}{2}\right\}=\frac{\sqrt{2}}{4}$$
3.  The magnitude of z is the product of the magnitudes of \(\frac{1}{2}\) and \(e^{j \pi / 4}\). However, \(|\frac{1}{2}|=\frac{1}{2}\) while \(|e^{j \theta}|=1\) for all \(\theta\). Thus,
    $$|z|=\left|\frac{1}{2} e^{j \pi / 4}\right|=\left|\frac{1}{2}\right|\left|e^{j \pi / 4}\right|=\frac{1}{2} \cdot 1=\frac{1}{2}$$
4.  The argument of z is the sum of the arguments of \(\frac{1}{2}\) and \(e^{j \pi / 4}\). Since \(\measuredangle \frac{1}{2}=0\) and \(\measuredangle e^{j \theta}=\theta\) for all \(\theta\)
    $$\measuredangle z=\measuredangle\left(\frac{1}{2} e^{j \pi / 4}\right)=\measuredangle \frac{1}{2}+\measuredangle e^{j \pi / 4}=0+\frac{\pi}{4}=\frac{\pi}{4}$$
5.  The complex conjugate of z is the product of the complex conjugates of \(\frac{1}{2}\) and \(e^{j \pi / 4}\). Since \(\frac{1}{2}^{*}=\frac{1}{2}\) and \((e^{j \theta})^{*}=e^{-j \theta}\) for all \(\theta\),
    $$z^{*}=\left(\frac{1}{2} e^{j \pi / 4}\right)^{*}=\frac{1}{2}^{*}\left(e^{j \pi / 4}\right)^{*}=\frac{1}{2} e^{-j \pi / 4}$$
6.  \(z+z^{*}\) is given by
    $$z+z^{*}=\frac{1}{2} e^{j \pi / 4}+\frac{1}{2} e^{-j \pi / 4}=\frac{e^{j \pi / 4}+e^{-j \pi / 4}}{2}=\cos \frac{\pi}{4}=\frac{\sqrt{2}}{2}$$
    Alternatively,
    $$\operatorname{Re}\{z\}=\frac{z+z^{*}}{2}, \quad \text{or } z+z^{*}=2 \operatorname{Re}\{z\}=2 \frac{\sqrt{2}}{4}=\frac{\sqrt{2}}{2}$$

## S1.2
1.  Express z as \(z=\sigma+j \Omega\), where \(\operatorname{Re}\{z\}=\sigma\) and \(\operatorname{Im}\{z\}=\Omega\). Recall that \(z^{*}\) is the complex conjugate of z, or \(z^{*}=\sigma-j \Omega\). Then
    $$\frac{z+z^{*}}{2}=\frac{(\sigma+j \Omega)+(\sigma-j \Omega)}{2}=\frac{2 \sigma+0}{2}=\sigma$$
2.  Similarly,
    $$\frac{z-z^{*}}{2}=\frac{(\sigma+j \Omega)-(\sigma-j \Omega)}{2}=\frac{0+2 j \Omega}{2}=j \Omega$$

Signals and Systems S1-2

## S1.3
1.  Euler's relation states that \(e^{j \theta}=\cos \theta+j \sin \theta\). Therefore, \(e^{-j \theta}=\cos (-\theta)+j \sin (-\theta)\). But, \(\cos (-\theta)=\cos \theta\) and \(\sin (-\theta)=-\sin \theta\). Thus, \(e^{-j \theta}=\cos \theta-j \sin \theta\). Substituting,
    $$\frac{e^{j \theta}+e^{-j \theta}}{2}=\frac{(\cos \theta+j \sin \theta)+(\cos \theta-j \sin \theta)}{2}=\frac{2 \cos \theta}{2}=\cos \theta$$
2.  Similarly,
    $$\frac{e^{j \theta}-e^{-j \theta}}{2 j}=\frac{(\cos \theta+j \sin \theta)-(\cos \theta-j \sin \theta)}{2 j}=\frac{2 j \sin \theta}{2 j}=\sin \theta$$

## S1.4
1.  We first find the complex conjugate of \(z=r e^{j \theta}\). From Euler's relation, \(r e^{j \theta}=r\cos \theta+j r\sin \theta=z\). Thus,
    $$z^{*}=r \cos \theta-j r \sin \theta=r \cos \theta+j r(-sin \theta)$$
    But \(\cos \theta=\cos (-\theta)\) and \(-\sin \theta=\sin (-\theta)\). Thus,
    $$z^{*}=r \cos (-\theta)+j r \sin (-\theta)=r e^{-j \theta}$$
2.  $$z^{2}=\left(r e^{j \theta}\right)^{2}=r^{2}\left(e^{j \theta}\right)^{2}=r^{2} e^{j 2 \theta}$$
3.  $$j z=e^{j \pi / 2} r e^{j \theta}=r e^{j\left(\theta+(\pi / 2)\right)}$$
4.  $$z z^{*}=\left(r e^{j \theta}\right)\left(r e^{-j \theta}\right)=r^{2} e^{j(\theta-\theta)}=r^{2} \cdot 1$$
5.  $$\frac{z}{z^{*}}=\frac{r e^{j \theta}}{r e^{-j \theta}}=e^{j(\theta+\theta)}=e^{j 2 \theta}$$
6.  $$\frac{1}{z}=\frac{1}{r e^{j \theta}}=\frac{1}{r} e^{-j \theta}$$
7.  From part (a), we directly plot the result in Figure S1.4-1, noting that for \(z=r e^{j \theta}\), r is the radial distance to the origin and \(\theta\) is the angle counterclockwise subtended by the vector with the positive real axis.
    - Im{z} 3 jr/6 3 J, Re{z} -> Figure S1.4-1
    - Im{z}, Re{z} -> Figure S1.4-2 (ii)
    - Im{z}, \(z^2 = 4 e^{j\pi/3}\) 9 4 9, Re{z} -> Figure S1.4-3 (iii)
    - Im{z}, \(jz = 2 e^{j2\pi/3}\) 3 2 2π, Re{z} -> Figure S1.4-4 (iv)
    - Im{z}, \(zz^*=e10\), Re=1 -> Figure S1.4-5
    - Im{z}, z*, Re{z} -> Figure S1.4-6 (v)
    - Im{z}, π/6 Re{z} 3 2 1 3 \(-j\pi/6\) z 2 -> Figure S1.4-7

## S1.5
This problem shows a useful manipulation. Multiply by \(e^{+j \alpha / 2} e^{-j \alpha / 2}=1\), yielding
$$e^{+j \alpha / 2} e^{-j \alpha / 2}\left(1-e^{j \alpha}\right)=e^{j \alpha / 2}\left(e^{-j \alpha / 2}-e^{j \alpha / 2}\right)$$
Now we note that \(2 j \sin (-x)=-2 j\sin x=e^{-x}-e^{x}\). Therefore,
$$1-e^{j \alpha}=e^{j \alpha / 2}\left(-2 j \sin \frac{\alpha}{2}\right)$$
Finally, we convert \(-j\) to complex exponential notation, \(-j=e^{-j \pi / 2}\). Thus,
$$1-e^{j \alpha}=e^{j \alpha / 2}\left(2 e^{-j \pi / 2} \sin \frac{\alpha}{2}\right)=2 \sin \frac{\alpha}{2} e^{j[(\alpha-\pi) / 2]}$$

## S1.6
There are three things a linear scaling of the form \(x(a t+b)\) can do:
1.  reverse direction => a is negative
2.  stretch or compress the time axis => \(|a| ≠1\)
3.  time shifting => \(b ≠0\)
1.  This is just a time reversal.
    x(-t) 1 -3 0 -> Figure S1.6-1
    Note: Amplitude remains the same. Also, reversal occurs about \(t=0\)
2.  This is a shift in time. At \(t=-2\) the vertical portion occurs.
    x(t + 2) -> Figure S1.6-2
3.  A scaling by a factor of 2 occurs as well as a time shift.
    x(2t + 2) -1 1 2 -> Figure S1.6-3
    Note: \(a>1\) induces a compression.
4.  All three effects are combined in this linear scaling.
    x(1 -3t) 2 3 1 3 -> Figure S1.6-4

## S1.7
This should be a review of calculus.
1.  $$\int_{0}^{a} e^{-2 t} d t =-\left.\frac{1}{2} e^{-2 t}\right|_{0} ^{a}=-\frac{1}{2} e^{-2 a}-\left[-\frac{1}{2} e^{-2(0)}\right]=\frac{1}{2}-\frac{1}{2} e^{-2 a}$$
2.  $$\int_{2}^{\infty} e^{-3 t} d t=-\left.\frac{1}{3} e^{-3 t}\right|_{2} ^{\infty}=\lim _{t \to \infty}\left(-\frac{1}{3} e^{-3 t}\right)+\frac{1}{3} e^{-3(2)}$$
    Therefore,
    $$\int_{2}^{\infty} e^{-3 t} d t=0+\frac{1}{3} e^{-6}=\frac{1}{3} e^{-6}$$

---

MIT OpenCourseWare
[http://ocw.mit.edu](http://ocw.mit.edu)
Resource: Signals and Systems
Professor Alan V. Oppenheim

The following may not correspond to a particular course on MIT OpenCourseWare, but has been provided by the author as an individual learning resource.

For information about citing these materials or our Terms of Use, visit: [http://ocw.mit.edu/terms](http://ocw.mit.edu/terms)
